Added back naive proof

examples/metatheory/MiniValeSemantics.fst
@@ -316,6 +316,35 @@ let inst_ins (i:ins) : with_wp (Ins i) =
   QProc (Ins i) (wp_ins i) (hasWp_ins i)
 
 ////////////////////////////////////////////////////////////////////////////////
+//Instance for Mov
+////////////////////////////////////////////////////////////////////////////////
+let lemma_Move (s0:state) (dst:operand) (src:operand)
+  : Ghost (state * fuel)
+  (requires OReg? dst)
+  (ensures fun (sM, fM) ->
+    eval_code (Ins (Mov64 dst src)) fM s0 == Some sM /\
+    eval_operand dst sM == eval_operand src s0 /\
+    sM == update_state (OReg?.r dst) sM s0
+  )
+  =
+  let Some sM = eval_code (Ins (Mov64 dst src)) 0 s0 in
+  (sM, 0)
+
+////////////////////////////////////////////////////////////////////////////////
+//Instance for Add
+////////////////////////////////////////////////////////////////////////////////
+let lemma_Add (s0:state) (dst:operand) (src:operand) : Ghost (state * fuel)
+  (requires OReg? dst /\ eval_operand dst s0 + eval_operand src s0 < pow2_64)
+  (ensures fun (sM, fM) ->
+    eval_code (Ins (Add64 dst src)) fM s0 == Some sM /\
+    eval_operand dst sM == eval_operand dst s0 + eval_operand src s0 /\
+    sM == update_state (OReg?.r dst) sM s0
+  )
+  =
+  let Some sM = eval_code (Ins (Add64 dst src)) 0 s0 in
+  (sM, 0)
+
+////////////////////////////////////////////////////////////////////////////////
 //Running the VC generator using the F* normalizer
 ////////////////////////////////////////////////////////////////////////////////
 unfold
@@ -388,24 +417,24 @@ let state_eq (s0 s1:state) : Ghost Type0
   s0 Rdx == s1 Rdx
 
 #reset-options
-(* let lemma_Triple (s0:state) *)
-(*   : Ghost (state & fuel) *)
-(*     (requires *)
-(*       s0 Rax < 100) *)
-(*     (ensures fun (sM, f0) -> *)
-(*       eval_code (Block codes_Triple) f0 s0 == Some sM /\ *)
-(*       sM Rbx == 3 * s0 Rax /\ *)
-(*       sM `feq` update_state Rax sM (update_state Rbx sM s0)) = *)
-(* // Naive proof: *)
-(*   let b1 = codes_Triple in *)
-(*   let (s2, fc2) = lemma_Move s0 (OReg Rbx) (OReg Rax) in let b2 = Cons?.tl b1 in *)
-(*   let (s3, fc3) = lemma_Add s2 (OReg Rax) (OReg Rbx) in  let b3 = Cons?.tl b2 in *)
-(*   let (s4, fc4) = lemma_Add s3 (OReg Rbx) (OReg Rax) in  let b4 = Cons?.tl b3 in *)
-(*   let (sM, f4) = (s4, 0) in *)
-(*   let f3 = lemma_merge (Cons?.hd b3) b4 s3 fc4 s4 f4 sM in *)
-(*   let f2 = lemma_merge (Cons?.hd b2) b3 s2 fc3 s3 f3 sM in *)
-(*   let fM = lemma_merge (Cons?.hd b1) b2 s0 fc2 s2 f2 sM in *)
-(*   (sM, fM) *)
+let lemma_Triple (s0:state)
+  : Ghost (state & fuel)
+    (requires
+      s0 Rax < 100)
+    (ensures fun (sM, f0) ->
+      eval_code (Block codes_Triple) f0 s0 == Some sM /\
+      sM Rbx == 3 * s0 Rax /\
+      sM `feq` update_state Rax sM (update_state Rbx sM s0)) =
+// Naive proof:
+  let b1 = codes_Triple in
+  let (s2, fc2) = lemma_Move s0 (OReg Rbx) (OReg Rax) in let b2 = Cons?.tl b1 in
+  let (s3, fc3) = lemma_Add s2 (OReg Rax) (OReg Rbx) in  let b3 = Cons?.tl b2 in
+  let (s4, fc4) = lemma_Add s3 (OReg Rbx) (OReg Rax) in  let b4 = Cons?.tl b3 in
+  let (sM, f4) = (s4, 0) in
+  let f3 = lemma_merge (Cons?.hd b3) b4 s3 fc4 s4 f4 sM in
+  let f2 = lemma_merge (Cons?.hd b2) b3 s2 fc3 s3 f3 sM in
+  let fM = lemma_merge (Cons?.hd b1) b2 s0 fc2 s2 f2 sM in
+  (sM, fM)
 
 let lemma_Triple_opt (s0:state)
   : Ghost (state & fuel)
